Memory/Target/Semantics.v
@@ -1,13 +1,15 @@
 Require Import Arith ZArith Lia List Structures.Equalities.
 
 From Vrac.Lib Require Import Tactics Option Eqb Error.
-From Vrac.Memory Require Import MemoryType ExecutionMemoryModel Context.
+From Vrac.Memory Require Import MemoryType ExecutionMemoryModel Context
+  ObservationMemoryModel.
 From Vrac.Common Require Import Syntax Semantics.
 From Vrac.Target Require Import Syntax.
 
 Module Semantics(V : DecidableType)(B: Eqb.EQB)
   (Import EMM: ExecutionMemoryModel B)
   (Import Ctx: Context.SIG V B EMM)
+  (Import OMM: ObservationMemoryModel B)
   (Import CStx: Common.Syntax.SIG V)
   (Import Stx: Target.Syntax.SIG V CStx)
   (CSem: Common.Semantics.SIG V B EMM Ctx CStx).
@@ -15,69 +17,126 @@ Module Semantics(V : DecidableType)(B: Eqb.EQB)
   Import CStx.Types CStx.Expr Stx.Stmt CSem.
   
   (* TODO: explanation wrt. to the companion paper. *)
-  Inductive sseval : forall (C: context) (Γ: type_env) (s: stmt) (M2: mem)
-                      (Invariant: forall x b, C.(E) x = ⎣b⎦ -> M2 ⊨ b), Prop :=
+  Inductive seval : forall (C: context)(O: obs)(Γ: type_env) (s: stmt) (M2: mem)
+                       (O2: obs) (Invariant: forall x b, C.(E) x = ⎣b⎦ -> M2 ⊨ b), Prop :=
     
-  | S_skip: forall C Γ,
-      sseval C Γ SSkip C.(M) C.(wf)
+  | S_skip: forall C O Γ,
+      seval C O Γ SSkip C.(M) O C.(wf)
                                              
-  | S_assign: forall C Γ e1 e2 τ v b δ M2
+  | S_assign: forall C O Γ e1 e2 τ v b δ M2
       (Hstore: store(mtype τ, C.(M), b, δ, v) = ⎣M2⎦),
       Expr.check_type Γ e1 = Ok τ ->
       Expr.check_type Γ e2 = Ok τ ->
       eeval C Γ e2 v ->
       lveval C Γ e2 (b,δ) ->
-      sseval C Γ (SAssign e1 e2) M2 (wf_after_store Hstore)
+      seval C O Γ (SAssign e1 e2) M2 O (wf_after_store Hstore)
 
-  | S_malloc: forall C Γ e1 e2 τ n b δ b' M2 M3
+  | S_malloc: forall C O Γ e1 e2 τ n b δ b' M2 M3
                 (Halloc: alloc(C.(M), Z.to_nat n) = (b', M2))
                 (Hstore: store(mtype (TPtr τ), M2, b, δ, Ptr(b',0%Z)) = ⎣M3⎦),
       Expr.check_type Γ e1 = Ok (TPtr τ) ->
       eeval C Γ e2 (Int n) ->
       lveval C Γ e1 (b,δ) ->
-      sseval C Γ (SMalloc e1 e2) M3 (wf_after_malloc Halloc Hstore)
+      seval C O Γ (SMalloc e1 e2) M3 O (wf_after_malloc Halloc Hstore)
 
-  | S_free: forall C Γ e b M2
+  | S_free: forall C O Γ e b M2
               (Hfree: free(C.(M), b) = ⎣M2⎦)
               (Him: forall x, C.(E) x <> ⎣b⎦),
       eeval C Γ e (Ptr(b, 0%Z)) ->
-      sseval C Γ (SFree e) M2 (wf_after_free Hfree Him)
+      seval C O Γ (SFree e) M2 O (wf_after_free Hfree Him)
                                              
-  | S_seq: forall C Γ s1 s2 M2 Wf2 M3 Wf3,
-      sseval C Γ s1 M2 Wf2 ->
-      sseval {|E:=C.(E);M:=M2;inj:=C.(inj);wf:=Wf2|} Γ s2 M3 Wf3 ->
-      sseval C Γ (SSeq s1 s2) M3 Wf3
+  | S_seq: forall C Γ s1 s2 M2 Wf2 M3 Wf3 O O2 O3,
+      seval C O Γ s1 M2 O2 Wf2 ->
+      seval {|E:=C.(E);M:=M2;inj:=C.(inj);wf:=Wf2|} O2 Γ s2 M3 O3 Wf3 ->
+      seval C O Γ (SSeq s1 s2) M3 O3 Wf3
 
-  | S_if_false: forall C Γ e s1 s2 M2 Wf2,
+  | S_if_false: forall C Γ e s1 s2 M2 Wf2 O O2,
       eeval C Γ e (Int 0%Z) ->
-      sseval C Γ s2 M2 Wf2 ->
-      sseval C Γ (SIf e s1 s2) M2 Wf2
+      seval C O Γ s2 M2 O2 Wf2 ->
+      seval C O Γ (SIf e s1 s2) M2 O2 Wf2
 
-  | S_if_true: forall C Γ e s1 s2 M1 Wf1 n,
+  | S_if_true: forall C Γ e s1 s2 M1 Wf1 n O O1,
       eeval C Γ e (Int n) ->
       n <> 0%Z -> 
-      sseval C Γ s1 M1 Wf1 ->
-      sseval C Γ (SIf e s1 s2) M1 Wf1
+      seval C O Γ s1 M1 O1 Wf1 ->
+      seval C O Γ (SIf e s1 s2) M1 O1 Wf1 
 
-  | S_while_false: forall C Γ e s,
+  | S_while_false: forall C Γ e s O,
       eeval C Γ e (Int 0%Z) ->
-      sseval C Γ (SWhile e s) C.(M) C.(wf)
+      seval C O Γ (SWhile e s) C.(M) O C.(wf)
 
-  | S_while_true: forall C Γ e s n M2 Wf2 M3 Wf3,
+  | S_while_true: forall C Γ e s n M2 Wf2 M3 Wf3 O O2 O3,
       eeval C Γ e (Int n) ->
       n <> 0%Z ->
-      sseval C Γ s M2 Wf2 ->
-      sseval {|E:=C.(E);M:=M2;inj:=C.(inj);wf:=Wf2|} Γ (SWhile e s) M3 Wf3 -> 
-      sseval C Γ (SWhile e s) M3 Wf3
+      seval C O Γ s M2 O2 Wf2 ->
+      seval {|E:=C.(E);M:=M2;inj:=C.(inj);wf:=Wf2|} O2 Γ (SWhile e s) M3 O3 Wf3 -> 
+      seval C O Γ (SWhile e s) M3 O3 Wf3
 
-  | S_let: forall C1 Γ x τ s C2 M3 Wf3 M4
+  | S_let: forall C1 Γ x τ s C2 M3 Wf3 M4 O O3
      (Hdom: C1.(E) x = ϵ)
      (Halloc: C2 = alloc_var C1 x (sizeof(mtype τ)))
      (Hdealloc: ⎣M4⎦ = dealloc_var {|E:=C2.(E);M:=M3;inj:=C2.(inj);wf:=Wf3|} x),
-      sseval C2 Γ s M3 Wf3 ->
-      sseval C1 Γ (SLet x τ s) M4 (wf_after_alloc_dealloc_var Hdom Halloc Hdealloc)
+      seval C2 O Γ s M3 O3 Wf3 ->
+      seval C1 O Γ (SLet x τ s) M4 O3
+        (wf_after_alloc_dealloc_var Hdom Halloc Hdealloc)
 
-  (* TODO: add missing rules *)
+  | S_assert: forall C O Γ e n,
+      eeval C Γ e (Int n) ->
+      n <> 0%Z ->
+      seval C O Γ (SAssert e) C.(M) O C.(wf)
+
+  | S_storeblock: forall C O Γ p e b n O2,
+      eeval C Γ p (Ptr(b,0%Z)) ->
+      eeval C Γ e (Int n) ->
+      store_block(O, b, Z.to_nat n) = O2 ->
+      seval C O Γ (SStoreblock p e) C.(M) O2 C.(wf)
+
+  | S_deleteblock: forall C O Γ p b O2,
+      eeval C Γ p (Ptr(b,0%Z)) ->
+      delete_block(O, b) = O2 ->
+      seval C O Γ (SDeleteblock p) C.(M) O2 C.(wf)
+
+  | S_initialize: forall C O Γ e τ b δ O2,
+      Expr.check_type Γ e = Ok (TPtr τ) ->
+      eeval C Γ e (Ptr(b,δ)) ->
+      initialize(mtype τ, O, b, δ) = O2 ->
+      seval C O Γ (SInitialize e) C.(M) O2 C.(wf)
+
+  | S_baseaddr: forall C O Γ e1 e2 τ b1 δ1 b2 δ2 M2
+      (Hstore: store(mtype (TPtr τ), C.(M), b1, δ1, Ptr(b2, 0%Z)) = ⎣M2⎦),
+      Expr.check_type Γ e1 = Ok(TPtr τ) ->
+      lveval C Γ e1 (b1,δ1) ->
+      eeval C Γ e2 (Ptr(b2,δ2)) ->
+      seval C O Γ (SBaseaddress e1 e2) M2 O (wf_after_store Hstore)
+
+  | S_offset: forall C O Γ e1 e2 b1 δ1 b2 δ2 M2
+      (Hstore: store(i64, C.(M), b1, δ1, Int δ2) = ⎣M2⎦),
+      lveval C Γ e1 (b1,δ1) ->
+      eeval C Γ e2 (Ptr(b2,δ2)) ->
+      seval C O Γ (SOffset e1 e2) M2 O (wf_after_store Hstore)
+
+  | S_block_length: forall C O Γ e1 e2 b1 δ1 b2 δ2 M2 n
+      (Hstore: store(i64, C.(M), b1, δ1, Int n) = ⎣M2⎦),
+      lveval C Γ e1 (b1,δ1) ->
+      eeval C Γ e2 (Ptr(b2,δ2)) ->
+      length(O, b2) = n -> 
+      seval C O Γ (SBlocklength e1 e2) M2 O (wf_after_store Hstore)
+
+  | S_is_valid: forall C O Γ e1 e2 b1 δ1 b2 δ2 M2 τ β
+      (Hstore: store(i64, C.(M), b1, δ1, Int (Z.b2z β)) = ⎣M2⎦),
+      Expr.check_type Γ e2 = Ok(TPtr τ) ->
+      lveval C Γ e1 (b1,δ1) ->
+      eeval C Γ e2 (Ptr(b2,δ2)) ->
+      is_valid_access(mtype τ, O, b2, δ2)  = β -> 
+      seval C O Γ (SIsvalid e1 e2) M2 O (wf_after_store Hstore)
+
+  | S_is_initialized: forall C O Γ e1 e2 b1 δ1 b2 δ2 M2 τ β
+      (Hstore: store(i64, C.(M), b1, δ1, Int (Z.b2z β)) = ⎣M2⎦),
+      Expr.check_type Γ e2 = Ok(TPtr τ) ->
+      lveval C Γ e1 (b1,δ1) ->
+      eeval C Γ e2 (Ptr(b2,δ2)) ->
+      is_initialized((mtype τ), O, b2, δ2) = β -> 
+      seval C O Γ (SIsinitialized e1 e2) M2 O (wf_after_store Hstore)
   .
   
 End Semantics.
@@ -85,10 +144,11 @@ End Semantics.
 Module Type SIG(V : DecidableType)(B: Eqb.EQB)
   (Import EMM: ExecutionMemoryModel B)
   (Import Ctx: Context.SIG V B EMM)
+  (Import OMM: ObservationMemoryModel B)
   (Import CStx: Common.Syntax.SIG V)
   (Import Stx: Target.Syntax.SIG V CStx)
   (CSem: Common.Semantics.SIG V B EMM Ctx CStx).
 
-  Include Semantics V B EMM Ctx CStx Stx CSem.
+  Include Semantics V B EMM Ctx OMM CStx Stx CSem.
   
 End SIG.
